BourbakiLean2/Logic.lean
@@ -1,0 +1,9 @@
+
+variable {p q : Prop}
+theorem imp_iff_not_imp_not : (p → q) ↔ (¬ q → ¬ p) := by
+  constructor
+  · exact fun h h' h'' => h' (h h'')
+  · intro h h'
+    by_cases h'' : q
+    · exact h''
+    · exact (h h'' h').elim
