BourbakiLean2/Set/Defs.lean
@@ -269,3 +269,6 @@ elab "Sort*" : term => do
 elab "Type*" : term => do
   let u ← Lean.Meta.mkFreshLevelMVar
   Elab.Term.levelMVarToParam (.sort (.succ u))
+
+instance {α : Type u} : CoeSort (Set α) (Type u) where
+  coe x := Subtype (fun a => a ∈ x)
